[wip] Useful lemmas, mostly regarding memory

Generated/erc20shim/ERC20Shim/mapping_index_access_mapping_address_uint256_of_address_user.lean
@@ -3,6 +3,8 @@ import Clear.ReasoningPrinciple
 
 import Generated.erc20shim.ERC20Shim.mapping_index_access_mapping_address_uint256_of_address_gen
 
+import Generated.erc20shim.ERC20Shim.Predicate
+import Generated.erc20shim.ERC20Shim.Variables
 
 namespace Generated.erc20shim.ERC20Shim
 
@@ -10,13 +12,92 @@ section
 
 open Clear EVMState Ast Expr Stmt FunctionDefinition State Interpreter ExecLemmas OutOfFuelLemmas Abstraction YulNotation PrimOps ReasoningPrinciple Utilities 
 
-def A_mapping_index_access_mapping_address_uint256_of_address (dataSlot : Identifier) (slot key : Literal) (s₀ s₉ : State) : Prop :=
-  let s₁ := s₀ 🇪⟦ s₀.evm.mstore 0x00 (Address.ofUInt256 key) ⟧
-  let s₂ := s₁ 🇪⟦ s₁.evm.mstore 0x20 slot ⟧
-  match s₂.evm.keccak256 0x00 0x40 with
-  | some ⟨addr, evm⟩ => s₉ = s₂ 🇪⟦ evm ⟧⟦ dataSlot ↦ addr ⟧
-  | none => s₉.evm.hash_collision = True
+abbrev AddressMap := Finmap (λ _ : Address ↦ UInt256)
 
+def A_mapping_index_access_mapping_address_uint256_of_address (dataSlot : Identifier) (slot key : Literal) (s₀ s₉ : State) : Prop :=
+  let account := Address.ofUInt256 key
+  ∀ {map : AddressMap}, account ∈ map →
+  ∃ address,
+  s₀.evm.keccak_map.lookup [ ↑account , slot ] = some address ∧
+  some (s₀.evm.sload address) = map.lookup account →
+  s₉ = s₀ ⟦ dataSlot ↦ address ⟧
+
+  -- account ∈ erc20.balances →
+  -- ∃ address, s₀.evm.keccak_map.lookup [ ↑account,  ERC20Private.balances ] = some address →
+  -- s₉ = s₀ ⟦ dataSlot ↦ address ⟧ 
+
+  -- let s₁ := s₀ 🇪⟦ s₀.evm.mstore 0x00 (Address.ofUInt256 key) ⟧
+  -- let s₂ := s₁ 🇪⟦ s₁.evm.mstore 0x20 slot ⟧
+  -- match s₂.evm.keccak256 0x00 0x40 with
+  -- | some ⟨addr, evm⟩ => s₉ = s₂ 🇪⟦ evm ⟧⟦ dataSlot ↦ addr ⟧
+  -- | none => s₉ = s₂ 🇪⟦ s₂.evm.addHashCollision ⟧
+
+-- lemma mapping_of_ok {dataSlot : Identifier} {slot key : Literal} {s₀ s₉ : State}
+--   : A_mapping_index_access_mapping_address_uint256_of_address dataSlot slot key s₀ s₉ →
+--     isOk s₀ → isOk s₉ := by
+--   intro mapping s₀_ok
+--   unfold A_mapping_index_access_mapping_address_uint256_of_address at mapping
+
+--   have : s₀🇪⟦mstore s₀.evm 0 ↑↑(Address.ofUInt256 key)⟧.isOk := by
+--     rw [isOk_setEvm]
+--     assumption
+
+--   simp at mapping
+--   rw [ evm_get_set_of_isOk s₀_ok
+--      , evm_get_set_of_isOk this
+--      ] at mapping
+
+--   -- split at mapping
+--   -- <;> apply_fun isOk at mapping
+--   -- <;> try rw [ isOk_insert ] at mapping
+--   -- <;> [simp only [ isOk_setEvm ] at mapping; simp only [ isOk_setEvm ] at mapping]
+--   -- <;> exact mapping.to_iff.mpr s₀_ok
+
+--   split at mapping <;> apply_fun isOk at mapping
+--   · rw [ isOk_insert ] at mapping
+--     rw [ isOk_setEvm, isOk_setEvm, isOk_setEvm] at mapping
+--     exact mapping.to_iff.mpr s₀_ok
+--   · rw [ isOk_setEvm, isOk_setEvm, isOk_setEvm] at mapping
+--     exact mapping.to_iff.mpr s₀_ok
+
+-- lemma lookup_addr_fail {dataSlot : Identifier} {slot key : Literal} {s₀ s₉ : State}
+--   : A_mapping_index_access_mapping_address_uint256_of_address dataSlot slot key s₀ s₉ →
+--     s₉.evm.hash_collision = true → 
+--     s₉[dataSlot]!! = 0 := by
+--   intro r_addr h
+--   rcases s₀ with ⟨evm, varstore⟩ | _ | _ <;> [simp only; aesop_spec; aesop_spec]
+
+--   clr_funargs
+
+--   unfold A_mapping_index_access_mapping_address_uint256_of_address at r_addr
+--   simp at r_addr
+  
+--   sorry
+
+-- lemma lookup_addr_ok {dataSlot : Identifier} {slot key : Literal} {s₀ s₉ : State}
+--   : A_mapping_index_access_mapping_address_uint256_of_address dataSlot slot key s₀ s₉ →
+--     s₉.evm.hash_collision = false → 
+--     ∃ addr, s₉[dataSlot]!! = addr := by
+--   intro r_addr
+--   sorry
+
+  -- unfold A_mapping_index_access_mapping_address_uint256_of_address at r_addr
+  -- simp at r_addr
+  
+  
+  -- unfold setEvm at r_addr
+  -- simp at r_addr
+  -- generalize prep_def
+  --   : (mstore s₀.evm 0 ↑↑(Address.ofUInt256 key)).mstore 32 slot = state_prep
+  --   at r_addr
+
+  -- cases (b.evm.keccak256 0x00 0x40) with
+  -- | none =>
+
+  --   use 0
+  --   sorry
+  -- | some a => sorry
+  
 -- Helper reifications
 lemma shift_eq_size : Fin.shiftLeft (n := UInt256.size) 1 160 = Address.size := by
   constructor
@@ -26,27 +107,49 @@ lemma EVMAddrSize' {s : State} : (s, [Fin.shiftLeft 1 160]) = (s, [Address.size.
   exact shift_eq_size
 
 lemma mapping_index_access_mapping_address_uint256_of_address_abs_of_concrete {s₀ s₉ : State} {dataSlot slot key} :
-  Spec (mapping_index_access_mapping_address_uint256_of_address_concrete_of_code.1 dataSlot slot key) s₀ s₉ →
-  Spec (A_mapping_index_access_mapping_address_uint256_of_address dataSlot slot key) s₀ s₉ := by
-  unfold mapping_index_access_mapping_address_uint256_of_address_concrete_of_code A_mapping_index_access_mapping_address_uint256_of_address  
+  CollidingSpec (mapping_index_access_mapping_address_uint256_of_address_concrete_of_code.1 dataSlot slot key) s₀ s₉ →
+  CollidingSpec (A_mapping_index_access_mapping_address_uint256_of_address dataSlot slot key) s₀ s₉ := by
+  unfold mapping_index_access_mapping_address_uint256_of_address_concrete_of_code A_mapping_index_access_mapping_address_uint256_of_address
   rcases s₀ with ⟨evm, varstore⟩ | _ | _ <;> [simp only; aesop_spec; aesop_spec]
-  apply spec_eq
+  apply collision_spec_eq'
+  
+  intro noCollision hasFuel
+  
   clr_funargs
 
   rw [ EVMSub', EVMShl', EVMAddrSize' ]; simp
   rw [ Address.and_size_eq_ofUInt256 ]
   rw [ multifill_cons, multifill_nil ]
   simp
-
+  
   clr_varstore
 
-  generalize prep_def : (mstore evm 0 ↑↑(Address.ofUInt256 key)).mstore 32 slot = state_prep
+  generalize acconut_def : Address.ofUInt256 key = account
+  
+  intro prog erc20 account_mem_balances
+  
+  rcases (Finmap.mem_iff.mp account_mem_balances) with ⟨bal, h_bal⟩
+  sorry
+  -- use address
+  -- intro h_lookup
+  -- generalize prep_def : (mstore evm 0 ↑↑account).mstore 32 slot = state_prep
 
-  cases state_prep.keccak256 0 64
-  · aesop_spec
-  · simp
-    unfold setEvm State.insert
-    aesop_spec
+  -- have : Option.isSome $ state_prep.keccak256 0 64 := by
+  --   unfold keccak256
+  --   unfold mkInterval
+  --   unfold MachineState.lookupMemory
+  --   unfold_let
+ 
+  --   rw [ ← prep_def ]
+  --   unfold mstore updateMemory
+  --   sorry
+
+  -- cases this
+  -- · simp
+  --   sorry
+  -- · simp
+  --   unfold setEvm State.insert
+  --   aesop_spec
 
 end
 
