Generated/erc20shim/ERC20Shim/fun_totalSupply_user.lean
@@ -17,7 +17,20 @@ lemma fun_totalSupply_abs_of_concrete {s₀ s₉ : State} {var_ } :
   Spec (fun_totalSupply_concrete_of_code.1 var_ ) s₀ s₉ →
   Spec (A_fun_totalSupply var_ ) s₀ s₉ := by
   unfold fun_totalSupply_concrete_of_code A_fun_totalSupply
-  aesop_spec
+  rcases s₀ with ⟨evm, varstore⟩ | _ | _ <;> [simp only; aesop_spec; aesop_spec]
+  apply spec_eq  
+  clr_funargs
+  intro hasFuel
+
+  unfold reviveJump
+  simp
+
+  rw [ ← State.insert_of_ok,  ← State.insert_of_ok,  ← State.insert_of_ok ]  
+  clr_varstore
+  intro h
+  unfold ERC20Private; dsimp only
+  symm
+  assumption
 
 end
 
